theory/Util/IntMap.v
@@ -1,8 +1,12 @@
+Require Import Arith.
+Require Import ZArith.
 Require Import Lia.
 Require Import List.
 Import ListNotations.
 Require Import PrimInt63.
 Require Import Uint63.
+
+Require Import Coq.Sorting.Permutation.
 
 Require Import Games.Util.Dec.
 Require Import TBGen.Util.IntHash.
@@ -16,20 +20,122 @@ Class IntMap (M : Type -> Type) : Type := {
   empty {X} : M X;
   add {X} : int -> X -> M X -> M X;
   lookup {X} : int -> M X -> option X;
+  to_list {X} : M X -> list (int * X);
   size {X} : M X -> nat;
 
   lookup_empty {X} : forall k, lookup k (empty : M X) = None;
+
   lookup_add {X} : forall k (x : X) m, lookup k (add k x m) = Some x;
   lookup_add_neq {X} : forall k k' (x : X) m, k <> k' ->
     lookup k (add k' x m) = lookup k m;
-  size_empty {X} : size (empty : M X) = 0;
-  size_add {X} : forall k (x : X) m,
-    size (add k x m) =
-      match lookup k m with
-      | Some _ => size m
-      | None => S (size m)
-      end
+
+  to_list_lookup {X} : forall (m : M X) k v, In (k,v) (to_list m) -> lookup k m = Some v;
+  lookup_to_list {X} : forall (m : M X) k v, lookup k m = Some v -> In (k,v) (to_list m);
+
+  to_list_NoDup_keys {X} : forall (m : M X), NoDup (map fst (to_list m));
+
+  size_to_list {X} : forall (m : M X), size m = length (to_list m);
   }.
+
+Lemma to_list_empty {M} `{IntMap M} {X} :
+  to_list (empty : M X) = [].
+Proof.
+  destruct (to_list (empty : M X)) as [|[k v] l] eqn:Heq.
+  - auto.
+  - assert (lookup k empty = Some v) as pf.
+    { apply to_list_lookup.
+      rewrite Heq; now left.
+    }
+    rewrite lookup_empty in pf; discriminate.
+Qed.
+
+Lemma size_empty {M} `{IntMap M} {X} :
+  size (empty : M X) = 0.
+Proof.
+  rewrite size_to_list.
+  rewrite to_list_empty; auto.
+Qed.
+
+Lemma size_add {M} `{IntMap M} {X} :
+  forall k (v : X) m,
+    size (add k v m) =
+    match lookup k m with
+    | Some _ => size m
+    | None => S (size m)
+    end.
+Proof.
+  intros.
+  rewrite size_to_list.
+  destruct lookup eqn:Hlookup.
+  - rewrite size_to_list.
+    do 2 rewrite <- map_length with (f := fst).
+    apply Permutation_length.
+    apply NoDup_Permutation.
+    + apply to_list_NoDup_keys.
+    + apply to_list_NoDup_keys.
+    + intros k'; split; intro pf.
+      * destruct (eqb k k') eqn:Hkeys.
+        -- rewrite eqb_spec in Hkeys; subst.
+           apply lookup_to_list in Hlookup.
+           apply in_map with (f := fst) in Hlookup; auto.
+        -- rewrite eqb_false_spec in Hkeys.
+           rewrite in_map_iff in pf.
+           destruct pf as [[k'' v'] [Hv'1 Hv'2]]; subst.
+           apply to_list_lookup in Hv'2.
+           rewrite lookup_add_neq in Hv'2; auto.
+           apply lookup_to_list in Hv'2.
+           apply in_map; auto.
+      * destruct (eqb k k') eqn:Hkeys.
+        -- rewrite eqb_spec in Hkeys; subst.
+           rewrite in_map_iff.
+           exists (k', v); split; auto.
+           apply lookup_to_list.
+           apply lookup_add.
+        -- rewrite eqb_false_spec in Hkeys.
+           rewrite in_map_iff in *.
+           destruct pf as [[k'' v'] [Hv'1 Hv'2]]; subst.
+           exists (k'', v'); split; auto.
+           apply lookup_to_list.
+           rewrite lookup_add_neq; auto.
+           apply to_list_lookup; auto.
+  - rewrite size_to_list.
+    do 2 rewrite <- map_length with (f := fst).
+    transitivity (length (k :: map fst (to_list m))); auto.
+    apply Permutation_length.
+    apply NoDup_Permutation.
+    + apply to_list_NoDup_keys.
+    + constructor.
+      * intro pf.
+        rewrite in_map_iff in pf.
+        destruct pf as [[k' v'] [pf1 pf2]]; subst.
+        simpl in Hlookup.
+        apply to_list_lookup in pf2; congruence.
+      * apply to_list_NoDup_keys.
+    + intros k'; split; intro pf.
+      * destruct (eqb k k') eqn:Hkeys.
+        -- rewrite eqb_spec in Hkeys; subst.
+           now left.
+        -- rewrite eqb_false_spec in Hkeys.
+           right.
+           rewrite in_map_iff in *.
+           destruct pf as [[k'' v'] [pf1 pf2]]; subst.
+           exists (k'', v'); split; auto.
+           apply to_list_lookup in pf2.
+           rewrite lookup_add_neq in pf2; auto.
+           apply lookup_to_list; auto.
+      * destruct pf as [pf|pf]; subst.
+        -- rewrite in_map_iff.
+           exists (k', v); split; auto.
+           apply lookup_to_list.
+           apply lookup_add.
+        -- rewrite in_map_iff in *.
+           destruct pf as [[k'' v'] [pf1 pf2]].
+           exists (k'', v'); split; auto.
+           apply lookup_to_list.
+           apply to_list_lookup in pf2.
+           rewrite lookup_add_neq; auto.
+           congruence.
+Qed.
 
 Definition hash_add {M} {X Y} `{IntMap M} `{IntHash X} :
   X -> Y -> M Y -> M Y :=
@@ -82,40 +188,6 @@ Fixpoint hash_adds {M} {X Y} `{IntMap M} `{IntHash X}
   | [] => m
   | (x,y) :: qs => hash_adds qs (hash_add x y m)
   end.
-
-Inductive good {M} {X Y} `{IntMap M} `{IntHash X} : M Y -> Prop :=
-  | good_e : good empty
-  | good_a {x y m} : good m -> hash_lookup x m = None -> good (hash_add x y m).
-
-Fixpoint good_as {M} {X Y} `{IntMap M} `{IntHash X} {ps : list (X * Y)}
-  {m : M Y} (pf : good m) (nd : NoDup (map fst ps))
-  (disj : forall x y, In (x,y) ps -> hash_lookup x m = None) {struct ps}
-  : good (hash_adds ps m).
-Proof.
-  induction ps as [|[x y] qs].
-  - exact pf.
-  - simpl.
-    apply good_as.
-    + apply good_a; auto.
-      apply (disj x y); now left.
-    + now inversion nd.
-    + intros x' y' HIn.
-      rewrite hash_lookup_add_neq.
-      * apply (disj x' y'); now right.
-      * simpl in nd; inversion nd.
-        intro Heq.
-        apply H3.
-        rewrite <- Heq.
-        rewrite in_map_iff.
-        exists (x', y'); split; auto.
-Qed.
-
-Record map_list_equiv {M} {X Y} `{IntMap M} `{IntHash X}
-  (m : M Y) (ps : list (X * Y)) : Prop := {
-  to_list_size : size m = List.length ps;
-  keys_unique : NoDup (map fst ps);
-  lookup_in {x y} : hash_lookup x m = Some y <-> In (x,y) ps;
-  }.
 
 Lemma hash_adds_add {M} {X Y} `{IntMap M} `{IntHash X}
   {ps : list (X * Y)} : forall x y m,
@@ -221,48 +293,6 @@ Proof.
            now rewrite Hx'x in n.
 Defined.
 
-Lemma good_to_list {M} {X Y} `{IntHash X} `{IntMap M}
-  (m : M Y) (g : good m) : exists (ps : list (X * Y)), map_list_equiv m ps.
-Proof.
-  induction g.
-  - exists nil; constructor.
-    + now rewrite size_empty.
-    + constructor.
-    + intros x y.
-      unfold hash_lookup.
-      now rewrite lookup_empty.
-  - destruct IHg as [ps [tl_sz key_un l_in]].
-    exists ((x,y) :: ps); constructor.
-    + unfold hash_add.
-      unfold hash_lookup in H1.
-      rewrite size_add.
-      rewrite H1.
-      simpl; congruence.
-    + simpl; constructor; auto.
-      intro HIn.
-      rewrite in_map_iff in HIn.
-      destruct HIn as [[str x'] [Hx1 Hx2]].
-      simpl in *.
-      rewrite Hx1 in Hx2.
-      rewrite <- l_in in Hx2; congruence.
-    + intros.
-      unfold hash_lookup, hash_add.
-      destruct (eq_dec (hash x0) (hash x)).
-      * rewrite e.
-        rewrite lookup_add.
-        split; intro.
-        -- pose (hash_inj _ _ e).
-           left; congruence.
-        -- destruct H2; [congruence|].
-           rewrite <- l_in in H2.
-           pose (hash_inj _ _ e); congruence.
-      * rewrite lookup_add_neq; auto.
-        unfold hash_lookup in l_in.
-        rewrite l_in.
-        split; intro; [now right|].
-        destruct H2; [congruence|auto].
-Qed.
-
 Lemma hash_lookup_adds_None_invert {M} {X Y} `{IntMap M} `{IntHash X}
   {ps} : forall {m : M Y} {x : X},
   hash_lookup x (hash_adds ps m) = None ->
@@ -345,13 +375,16 @@ Global Instance AssocList_SM : IntMap (AL.t int) := {|
   empty X := AL.empty;
   add X := AL.add;
   lookup X := AL.lookup;
+  to_list X := AL.to_list;
   size X := AL.size;
 
   lookup_empty X := AL.lookup_empty;
   lookup_add X := AL.lookup_add;
   lookup_add_neq X := AL.lookup_add_neq;
-  size_empty X := AL.size_empty;
-  size_add X := AL.size_add;
+  to_list_lookup X := AL.to_list_lookup;
+  lookup_to_list X := AL.lookup_to_list;
+  to_list_NoDup_keys X := AL.to_list_NoDup_keys;
+  size_to_list X := AL.size_to_list;
   |}.
 
 Section CondHashFacts.
@@ -410,47 +443,6 @@ Fixpoint chash_adds (ps : list (X * Y)) (m : M Y) {struct ps} : M Y :=
   | [] => m
   | (x,y) :: qs => chash_adds qs (chash_add x y m)
   end.
-
-Inductive cgood : M Y -> Prop :=
-  | cgood_e : cgood empty
-  | cgood_a {x y m} : P x -> cgood m -> chash_lookup x m = None -> cgood (chash_add x y m).
-
-Fixpoint cgood_as {ps : list (X * Y)}
-  {m : M Y} (pf : cgood m) (nd : NoDup (map fst ps))
-  (pps : Forall P (map fst ps))
-  (disj : forall x y, In (x,y) ps -> chash_lookup x m = None) {struct ps}
-  : cgood (chash_adds ps m).
-Proof.
-  induction ps as [|[x y] qs].
-  - exact pf.
-  - inversion pps.
-    simpl.
-    apply cgood_as; auto.
-    + apply cgood_a; auto.
-      apply (disj x y); now left.
-    + now inversion nd.
-    + intros x' y' HIn.
-      rewrite chash_lookup_add_neq; auto.
-      * apply (disj x' y'); now right.
-      * simpl in nd; inversion nd.
-        intro Heq.
-        apply H7.
-        rewrite <- Heq.
-        rewrite in_map_iff.
-        exists (x', y'); split; auto.
-      * rewrite Forall_forall in H4.
-        apply H4.
-        apply in_map with (f := fst) in HIn.
-        auto.
-Qed.
-
-Record cmap_list_equiv (m : M Y) (ps : list (X * Y)) : Prop := {
-  cto_list_size : size m = List.length ps;
-  all_P : Forall P (map fst ps);
-  ckeys_unique : NoDup (map fst ps);
-  clookup_in {x y} : chash_lookup x m = Some y <-> exists x',
-    chash x = chash x' /\ In (x',y) ps;
-  }.
 
 Lemma chash_adds_add {ps : list (X * Y)} : forall x y m,
   chash_add x y (chash_adds ps m) = chash_adds (ps ++ [(x,y)]) m.
@@ -568,61 +560,6 @@ Proof.
         rewrite lookup_add_neq in pf; auto.
 Defined.
 
-Lemma cgood_to_list (m : M Y) (g : cgood m) : exists (ps : list (X * Y)),
-  cmap_list_equiv m ps.
-Proof.
-  induction g.
-  - exists nil; constructor.
-    + now rewrite size_empty.
-    + constructor.
-    + constructor.
-    + intros x y.
-      unfold chash_lookup.
-      rewrite lookup_empty.
-      split.
-      * congruence.
-      * intros [? [? []]].
-  - destruct IHg as [ps [tl_sz key_P key_un l_in]].
-    exists ((x,y) :: ps); constructor.
-    + unfold chash_add.
-      unfold chash_lookup in H2.
-      rewrite size_add.
-      rewrite H2.
-      simpl; congruence.
-    + constructor; auto.
-    + simpl; constructor; auto.
-      intro HIn.
-      rewrite in_map_iff in HIn.
-      destruct HIn as [[str x'] [Hx1 Hx2]].
-      simpl in *.
-      rewrite Hx1 in Hx2.
-      assert (exists y, chash x = chash y /\ In (y, x') ps) as pf.
-      { exists x; split; auto. }
-      rewrite <- l_in in pf.
-      rewrite H2 in pf.
-      congruence.
-    + intros.
-      unfold chash_lookup, chash_add.
-      destruct (eq_dec (chash x0) (chash x)).
-      * rewrite e.
-        rewrite lookup_add.
-        split; intro.
-        -- exists x; split; auto; left; congruence.
-        -- destruct H3 as [x' [Hx'1 Hx'2]].
-           destruct Hx'2 as [|Hx'2]; [congruence|].
-           assert (exists y, chash x = chash y /\ In (y, y0) ps) as pf.
-           { exists x'; split; auto. }
-           rewrite <- l_in in pf.
-           rewrite H2 in pf; discriminate.
-      * rewrite lookup_add_neq; auto.
-        unfold chash_lookup in l_in.
-        rewrite l_in; auto.
-        split; intros [x' [Hx'1 Hx'2]].
-        -- exists x'; split; auto; now right.
-        -- destruct Hx'2; [congruence|].
-           exists x'; auto.
-Defined.
-
 Lemma chash_lookup_adds_None_invert {ps} (pps : Forall P (map fst ps)) : forall {m : M Y} {x : X}, P x ->
   chash_lookup x (chash_adds ps m) = None ->
   (~ In x (List.map fst ps)) /\
@@ -702,3 +639,96 @@ Proof.
 Qed.
 
 End CondHashFacts.
+
+Definition to_nat (i : int) : nat :=
+  Z.to_nat (to_Z i).
+
+Lemma to_nat_inj (i j : int) :
+  to_nat i = to_nat j -> i = j.
+Proof.
+  unfold to_nat; intro pf.
+  apply Z2Nat.inj in pf.
+  - apply to_Z_inj; auto.
+  - apply to_Z_bounded.
+  - apply to_Z_bounded.
+Qed.
+
+Lemma to_nat_bound (i : int) :
+  to_nat i < 2^63.
+Proof.
+  unfold to_nat.
+  assert (2^63 = Z.to_nat (2^63)%Z) as pf.
+  { rewrite Z2Nat.inj_pow; try lia.
+    reflexivity.
+  }
+  rewrite pf.
+  rewrite <- Z2Nat.inj_lt.
+  - apply to_Z_bounded.
+  - apply to_Z_bounded.
+  - lia.
+Qed.
+
+Lemma NoDup_nat_length_bound n : forall (l : list nat),
+  NoDup l -> Forall (fun x => x < n) l ->
+  length l <= n.
+Proof.
+  induction n; intros l nd Hl.
+  - destruct l as [|x l'].
+    + simpl; lia.
+    + apply Forall_inv in Hl; lia.
+  - destruct (in_dec n l) as [Hin|Hnin].
+    + apply in_split in Hin.
+      destruct Hin as [l1 [l2 ?]]; subst.
+      rewrite app_length; simpl.
+      rewrite Nat.add_succ_r.
+      apply le_n_S.
+      rewrite <- app_length.
+      apply IHn.
+      * apply NoDup_remove_1 in nd; auto.
+      * apply NoDup_remove_2 in nd.
+        rewrite Forall_forall in *.
+        intros x Hx.
+        assert (x < S n) as pf.
+        { apply Hl.
+          apply in_or_app.
+          apply in_app_or in Hx.
+          destruct Hx.
+          -- now left.
+          -- now right; right.
+        }
+        assert (x <> n) by congruence; lia.
+    + apply le_S.
+      apply IHn; auto.
+      rewrite Forall_forall in *.
+      intros x Hx.
+      specialize (Hl x Hx).
+      inversion Hl.
+      * congruence.
+      * lia.
+Qed.
+
+Lemma NoDup_int_length_bound (l : list int) :
+  NoDup l -> length l <= (2^63).
+Proof.
+  intro nd.
+  rewrite <- map_length with (f := to_nat).
+  apply NoDup_nat_length_bound.
+  - apply FinFun.Injective_map_NoDup.
+    + exact to_nat_inj.
+    + exact nd.
+  - rewrite Forall_forall.
+    intros x Hx.
+    rewrite in_map_iff in Hx.
+    destruct Hx as [i [Hi _]].
+    rewrite <- Hi.
+    apply to_nat_bound.
+Qed.
+
+Lemma size_bound {M} `{IntMap M} {X} (m : M X) :
+  size m <= (2^63).
+Proof.
+  rewrite size_to_list.
+  rewrite <- map_length with (f := fst).
+  apply NoDup_int_length_bound.
+  apply to_list_NoDup_keys.
+Qed.
